bench-hybrid/coqfiles/imp.v
@@ -1,14 +1,13 @@
-
-Require Import Minuska.pval_ocaml_binding Minuska.default_everything Minuska.builtin.empty Minuska.builtin.klike Minuska.pi.trivial.
+Require Import Minuska.pval_ocaml_binding Minuska.builtin.klike Minuska.pi.trivial Minuska.default_everything.
 Definition mybeta := (bi_beta MyUnit builtins_klike).
 #[global] Existing Instance mybeta.
 Definition my_program_info := trivial.MyProgramInfo.
 Definition mysigma : StaticModel := (default_everything.DSM my_program_info).
 Existing Instance mysigma.
-#[global] Existing Instance pi.trivial.MyProgramInfo.
+#[global] Existing Instance my_program_info.
 Definition myContext := (context-template (@t_term _ _ "c" [(HOLE); (t_over (notations.inject_variable "STATE"))]) with HOLE).
-Definition isValue (X : Expression2) := (mkSideCondition _ b_cond_is_true [(e_fun b_bool_or [(e_fun b_isZ [(X)]); (e_fun b_bool_or [(e_fun b_isBool [(X)]); (e_fun b_bool_or [(e_fun b_have_same_symbol [(X); (e_ground (@t_term symbol builtin_value "unitValue" []))]); (e_fun b_isString [(X)])])])])]).
-Definition isNonValue (X : Expression2) := (mkSideCondition _ b_cond_is_true [(e_fun b_bool_neg [(e_fun b_bool_or [(e_fun b_isZ [(X)]); (e_fun b_bool_or [(e_fun b_isBool [(X)]); (e_fun b_bool_or [(e_fun b_have_same_symbol [(X); (e_ground (@t_term symbol builtin_value "unitValue" []))]); (e_fun b_isString [(X)])])])])])]).
+Definition isValue (X : Expression2) := (sc_or (sc_atom b_isZ [(X)])(sc_or (sc_atom b_isString [(X)])(sc_or (sc_atom b_isBool [(X)])(sc_atom b_have_same_symbol [(X); (e_ground (@t_term symbol builtin_value "unitValue" []))])))).
+#[export] Instance isValue_nsc (X : Expression2) : NegableSideCondition (isValue X) := ltac:(intros; unfold isValue in *; apply _).
 
 
 #[local]
@@ -18,34 +17,33 @@ Instance LangDefaults : Defaults := {|
     default_context_template := myContext ;
 
     default_isValue := isValue ;
-    default_isNonValue := isNonValue ;
 |}.
 
 Definition frame_simple : (variable*(TermOver BuiltinOrVar)) := ("X",(@t_term symbol BuiltinOrVar "c" [(@t_term symbol BuiltinOrVar "builtin.cseq" [(t_over (bov_variable "X")); (t_over (bov_variable "REST"))]); (t_over (bov_variable "STATE"))])).
 Definition Lang_Decls : list Declaration := [
-(decl_strict (mkStrictnessDeclaration _ "plus" 2 [0; 1] isValue isNonValue myContext))
-;(decl_strict (mkStrictnessDeclaration _ "minus" 2 [0; 1] isValue isNonValue myContext))
-;(decl_strict (mkStrictnessDeclaration _ "assign" 2 [1] isValue isNonValue myContext))
-;(decl_strict (mkStrictnessDeclaration _ "seq" 2 [0] isValue isNonValue myContext))
-;(decl_strict (mkStrictnessDeclaration _ "ite" 3 [0] isValue isNonValue myContext))
-;(decl_strict (mkStrictnessDeclaration _ "eq" 2 [0; 1] isValue isNonValue myContext))
-;(decl_strict (mkStrictnessDeclaration _ "le" 2 [0; 1] isValue isNonValue myContext))
-;(decl_strict (mkStrictnessDeclaration _ "lt" 2 [0; 1] isValue isNonValue myContext))
-;(decl_strict (mkStrictnessDeclaration _ "neg" 1 [0] isValue isNonValue myContext))
+(decl_strict (mkStrictnessDeclaration _ "plus" 2 [0; 1] isValue _ myContext))
+;(decl_strict (mkStrictnessDeclaration _ "minus" 2 [0; 1] isValue _ myContext))
+;(decl_strict (mkStrictnessDeclaration _ "assign" 2 [1] isValue _ myContext))
+;(decl_strict (mkStrictnessDeclaration _ "seq" 2 [0] isValue _ myContext))
+;(decl_strict (mkStrictnessDeclaration _ "ite" 3 [0] isValue _ myContext))
+;(decl_strict (mkStrictnessDeclaration _ "eq" 2 [0; 1] isValue _ myContext))
+;(decl_strict (mkStrictnessDeclaration _ "le" 2 [0; 1] isValue _ myContext))
+;(decl_strict (mkStrictnessDeclaration _ "lt" 2 [0; 1] isValue _ myContext))
+;(decl_strict (mkStrictnessDeclaration _ "neg" 1 [0] isValue _ myContext))
 ] ++ [
-(basic_rule my_program_info "init" (@t_term symbol BuiltinOrVar "builtin.init" []) (@t_term symbol Expression2 "c" [(@t_term symbol Expression2 "builtin.cseq" [(@t_over symbol Expression2(e_query qs_program [])); (@t_term symbol Expression2 "builtin.empty_cseq" [])]); (@t_over symbol Expression2(e_fun b_map_empty []))]) [])
-; (framed_rule my_program_info frame_simple "aexpr.plus" (@t_term symbol BuiltinOrVar "plus" [(t_over (bov_variable "X")); (t_over (bov_variable "Y"))]) (@t_over symbol Expression2(e_fun b_Z_plus [(e_variable "X"); (e_variable "Y")])) [(mkSideCondition _ b_cond_is_true [(e_fun b_isZ [(e_variable "X")])]); (mkSideCondition _ b_cond_is_true [(e_fun b_isZ [(e_variable "Y")])])])
-; (framed_rule my_program_info frame_simple "aexpr.minus" (@t_term symbol BuiltinOrVar "minus" [(t_over (bov_variable "X")); (t_over (bov_variable "Y"))]) (@t_over symbol Expression2(e_fun b_Z_minus [(e_variable "X"); (e_variable "Y")])) [(mkSideCondition _ b_cond_is_true [(e_fun b_isZ [(e_variable "X")])]); (mkSideCondition _ b_cond_is_true [(e_fun b_isZ [(e_variable "Y")])])])
-; (basic_rule my_program_info "var.assign" (@t_term symbol BuiltinOrVar "c" [(@t_term symbol BuiltinOrVar "builtin.cseq" [(@t_term symbol BuiltinOrVar "assign" [(t_over (bov_variable "X")); (t_over (bov_variable "V"))]); (t_over (bov_variable "REST"))]); (t_over (bov_variable "STATE"))]) (@t_term symbol Expression2 "c" [(@t_term symbol Expression2 "builtin.cseq" [(@t_term symbol Expression2 "unitValue" []); (@t_over symbol Expression2(e_variable "REST"))]); (@t_over symbol Expression2(e_fun b_map_update [(e_variable "STATE"); (e_variable "X"); (e_variable "V")]))]) [(mkSideCondition _ b_cond_is_true [(e_fun b_have_same_symbol [(e_variable "X"); (e_ground (@t_term symbol builtin_value "var" []))])]); (mkSideCondition _ b_cond_is_true [(e_fun b_bool_or [(e_fun b_isZ [(e_variable "V")]); (e_fun b_isString [(e_variable "V")])])])])
-; (basic_rule my_program_info "var.lookup" (@t_term symbol BuiltinOrVar "c" [(@t_term symbol BuiltinOrVar "builtin.cseq" [(t_over (bov_variable "X")); (t_over (bov_variable "REST"))]); (t_over (bov_variable "STATE"))]) (@t_term symbol Expression2 "c" [(@t_term symbol Expression2 "builtin.cseq" [(@t_over symbol Expression2(e_fun b_map_lookup [(e_variable "STATE"); (e_variable "X")])); (@t_over symbol Expression2(e_variable "REST"))]); (@t_over symbol Expression2(e_variable "STATE"))]) [(mkSideCondition _ b_cond_is_true [(e_fun b_have_same_symbol [(e_variable "X"); (e_ground (@t_term symbol builtin_value "var" []))])])])
-; (framed_rule my_program_info frame_simple "stmt.seq" (@t_term symbol BuiltinOrVar "seq" [(@t_term symbol BuiltinOrVar "unitValue" []); (t_over (bov_variable "X"))]) (@t_over symbol Expression2(e_variable "X")) [])
-; (framed_rule my_program_info frame_simple "bexpr.eq" (@t_term symbol BuiltinOrVar "eq" [(t_over (bov_variable "X")); (t_over (bov_variable "Y"))]) (@t_over symbol Expression2(e_fun b_Z_eq [(e_variable "X"); (e_variable "Y")])) [(mkSideCondition _ b_cond_is_true [(e_fun b_isZ [(e_variable "X")])]); (mkSideCondition _ b_cond_is_true [(e_fun b_isZ [(e_variable "Y")])])])
-; (framed_rule my_program_info frame_simple "bexpr.le" (@t_term symbol BuiltinOrVar "le" [(t_over (bov_variable "X")); (t_over (bov_variable "Y"))]) (@t_over symbol Expression2(e_fun b_Z_isLe [(e_variable "X"); (e_variable "Y")])) [(mkSideCondition _ b_cond_is_true [(e_fun b_isZ [(e_variable "X")])]); (mkSideCondition _ b_cond_is_true [(e_fun b_isZ [(e_variable "Y")])])])
-; (framed_rule my_program_info frame_simple "bexpr.lt" (@t_term symbol BuiltinOrVar "lt" [(t_over (bov_variable "X")); (t_over (bov_variable "Y"))]) (@t_over symbol Expression2(e_fun b_Z_isLt [(e_variable "X"); (e_variable "Y")])) [(mkSideCondition _ b_cond_is_true [(e_fun b_isZ [(e_variable "X")])]); (mkSideCondition _ b_cond_is_true [(e_fun b_isZ [(e_variable "Y")])])])
-; (framed_rule my_program_info frame_simple "bexpr.neg" (@t_term symbol BuiltinOrVar "not" [(t_over (bov_variable "X"))]) (@t_over symbol Expression2(e_fun b_bool_neg [(e_variable "X")])) [(mkSideCondition _ b_cond_is_true [(e_fun b_isBool [(e_variable "X")])])])
-; (framed_rule my_program_info frame_simple "stmt.ite.true" (@t_term symbol BuiltinOrVar "ite" [(t_over (bov_variable "B")); (t_over (bov_variable "X")); (t_over (bov_variable "Y"))]) (@t_over symbol Expression2(e_variable "X")) [(mkSideCondition _ b_cond_is_true [(e_fun b_isBool [(e_variable "B")])]); (mkSideCondition _ b_cond_is_true [(e_fun b_bool_eq [(e_variable "B"); (e_fun b_true [])])])])
-; (framed_rule my_program_info frame_simple "stmt.ite.false" (@t_term symbol BuiltinOrVar "ite" [(t_over (bov_variable "B")); (t_over (bov_variable "X")); (t_over (bov_variable "Y"))]) (@t_over symbol Expression2(e_variable "Y")) [(mkSideCondition _ b_cond_is_true [(e_fun b_isBool [(e_variable "B")])]); (mkSideCondition _ b_cond_is_true [(e_fun b_bool_eq [(e_variable "B"); (e_fun b_false [])])])])
-; (framed_rule my_program_info frame_simple "while.unfold" (@t_term symbol BuiltinOrVar "while" [(t_over (bov_variable "B")); (t_over (bov_variable "S"))]) (@t_term symbol Expression2 "ite" [(@t_over symbol Expression2(e_variable "B")); (@t_term symbol Expression2 "seq" [(@t_over symbol Expression2(e_variable "S")); (@t_term symbol Expression2 "while" [(@t_over symbol Expression2(e_variable "B")); (@t_over symbol Expression2(e_variable "S"))])]); (@t_term symbol Expression2 "unitValue" [])]) [])
+(basic_rule my_program_info "init" (@t_term symbol BuiltinOrVar "builtin.init" []) (@t_term symbol Expression2 "c" [(@t_term symbol Expression2 "builtin.cseq" [(@t_over symbol Expression2(e_query qs_program [])); (@t_term symbol Expression2 "builtin.empty_cseq" [])]); (@t_over symbol Expression2(e_fun b_map_empty []))]) sc_true)
+; (framed_rule my_program_info frame_simple "aexpr.plus" (@t_term symbol BuiltinOrVar "plus" [(t_over (bov_variable "X")); (t_over (bov_variable "Y"))]) (@t_over symbol Expression2(e_fun b_Z_plus [(e_variable "X"); (e_variable "Y")])) (sc_and (sc_atom b_isZ [(e_variable "X")])(sc_atom b_isZ [(e_variable "Y")])))
+; (framed_rule my_program_info frame_simple "aexpr.minus" (@t_term symbol BuiltinOrVar "minus" [(t_over (bov_variable "X")); (t_over (bov_variable "Y"))]) (@t_over symbol Expression2(e_fun b_Z_minus [(e_variable "X"); (e_variable "Y")])) (sc_and (sc_atom b_isZ [(e_variable "X")])(sc_atom b_isZ [(e_variable "Y")])))
+; (basic_rule my_program_info "var.assign" (@t_term symbol BuiltinOrVar "c" [(@t_term symbol BuiltinOrVar "builtin.cseq" [(@t_term symbol BuiltinOrVar "assign" [(t_over (bov_variable "X")); (t_over (bov_variable "V"))]); (t_over (bov_variable "REST"))]); (t_over (bov_variable "STATE"))]) (@t_term symbol Expression2 "c" [(@t_term symbol Expression2 "builtin.cseq" [(@t_term symbol Expression2 "unitValue" []); (@t_over symbol Expression2(e_variable "REST"))]); (@t_over symbol Expression2(e_fun b_map_update [(e_variable "STATE"); (e_variable "X"); (e_variable "V")]))]) (sc_and (sc_atom b_have_same_symbol [(e_variable "X"); (e_ground (@t_term symbol builtin_value "var" []))])(sc_or (sc_atom b_isZ [(e_variable "V")])(sc_atom b_isString [(e_variable "V")]))))
+; (basic_rule my_program_info "var.lookup" (@t_term symbol BuiltinOrVar "c" [(@t_term symbol BuiltinOrVar "builtin.cseq" [(t_over (bov_variable "X")); (t_over (bov_variable "REST"))]); (t_over (bov_variable "STATE"))]) (@t_term symbol Expression2 "c" [(@t_term symbol Expression2 "builtin.cseq" [(@t_over symbol Expression2(e_fun b_map_lookup [(e_variable "STATE"); (e_variable "X")])); (@t_over symbol Expression2(e_variable "REST"))]); (@t_over symbol Expression2(e_variable "STATE"))]) (sc_atom b_have_same_symbol [(e_variable "X"); (e_ground (@t_term symbol builtin_value "var" []))]))
+; (framed_rule my_program_info frame_simple "stmt.seq" (@t_term symbol BuiltinOrVar "seq" [(@t_term symbol BuiltinOrVar "unitValue" []); (t_over (bov_variable "X"))]) (@t_over symbol Expression2(e_variable "X")) sc_true)
+; (framed_rule my_program_info frame_simple "bexpr.eq" (@t_term symbol BuiltinOrVar "eq" [(t_over (bov_variable "X")); (t_over (bov_variable "Y"))]) (@t_over symbol Expression2(e_fun b_Z_eq [(e_variable "X"); (e_variable "Y")])) (sc_and (sc_atom b_isZ [(e_variable "X")])(sc_atom b_isZ [(e_variable "Y")])))
+; (framed_rule my_program_info frame_simple "bexpr.le" (@t_term symbol BuiltinOrVar "le" [(t_over (bov_variable "X")); (t_over (bov_variable "Y"))]) (@t_over symbol Expression2(e_fun b_Z_isLe [(e_variable "X"); (e_variable "Y")])) (sc_and (sc_atom b_isZ [(e_variable "X")])(sc_atom b_isZ [(e_variable "Y")])))
+; (framed_rule my_program_info frame_simple "bexpr.lt" (@t_term symbol BuiltinOrVar "lt" [(t_over (bov_variable "X")); (t_over (bov_variable "Y"))]) (@t_over symbol Expression2(e_fun b_Z_isLt [(e_variable "X"); (e_variable "Y")])) (sc_and (sc_atom b_isZ [(e_variable "X")])(sc_atom b_isZ [(e_variable "Y")])))
+; (framed_rule my_program_info frame_simple "bexpr.neg" (@t_term symbol BuiltinOrVar "not" [(t_over (bov_variable "X"))]) (@t_over symbol Expression2(e_fun b_bool_neg [(e_variable "X")])) (sc_atom b_isBool [(e_variable "X")]))
+; (framed_rule my_program_info frame_simple "stmt.ite.true" (@t_term symbol BuiltinOrVar "ite" [(t_over (bov_variable "B")); (t_over (bov_variable "X")); (t_over (bov_variable "Y"))]) (@t_over symbol Expression2(e_variable "X")) (sc_and (sc_atom b_isBool [(e_variable "B")])(sc_atom b_bool_is_true [(e_variable "B")])))
+; (framed_rule my_program_info frame_simple "stmt.ite.false" (@t_term symbol BuiltinOrVar "ite" [(t_over (bov_variable "B")); (t_over (bov_variable "X")); (t_over (bov_variable "Y"))]) (@t_over symbol Expression2(e_variable "Y")) (sc_and (sc_atom b_isBool [(e_variable "B")])(sc_atom b_bool_is_false [(e_variable "B")])))
+; (framed_rule my_program_info frame_simple "while.unfold" (@t_term symbol BuiltinOrVar "while" [(t_over (bov_variable "B")); (t_over (bov_variable "S"))]) (@t_term symbol Expression2 "ite" [(@t_over symbol Expression2(e_variable "B")); (@t_term symbol Expression2 "seq" [(@t_over symbol Expression2(e_variable "S")); (@t_term symbol Expression2 "while" [(@t_over symbol Expression2(e_variable "B")); (@t_over symbol Expression2(e_variable "S"))])]); (@t_term symbol Expression2 "unitValue" [])]) sc_true)
 
 ].
 Definition T := Eval vm_compute in (to_theory Act (process_declarations Act default_act mybeta my_program_info Lang_Decls)). 
